Completed filter units

verification_finalised/bank/bank.dfy
@@ -78,6 +78,15 @@ class {:autocontracts} BloodBank {
         units := units[..index] + units[(index+1)..];
     }
 
+    // CheckAvailableUnits takes a criterion and a number of blood units and determines whether 
+    // the blood bank has enough units satisfying the criterion. The criterion is the same as specified 
+    // for OrderUnits
+    method CheckAvailableUnits(criterion: int, num: int) returns (result: bool)
+    ensures units == old(units)
+    {
+        
+    }
+
     // OrderUnits removes the specified number of blood units from the bank which satisfy
     // a particular criterion. If there are not enough units to meet the specified number, 
     // the maximum amount available is returned. In the real implementation, the criterion 
@@ -89,10 +98,26 @@ class {:autocontracts} BloodBank {
     {}
 
     // FilterUnits returns a sequence of all units in the blood bank which satisfy a particular 
-    // criterion. The criterion works in the same manner as the criterion for OrderUnits. 
-    // FilterUnits does not modifiy the blood bank units sequence.
-    method FilterUnits(criterion: int) returns (result: seq<int>)
-    {}
+    // criterion c. The criterion works in the same manner as the criterion for OrderUnits. 
+    // FilterUnits does not modifiy the blood bank units sequence. FilterUnits does not guarantee
+    // the order of the results
+    method FilterUnits(c: int) returns (results: seq<int>)
+    requires c != 0;
+    ensures units == old(units);
+    ensures forall i :: i in results <==> (i%c == 0 && i in units);
+    {
+        results := [];
+        var index, limit := 0, |units|;
+        
+        while index < limit
+        decreases limit - index;
+        invariant index <= limit;
+        invariant forall i :: i in results <==> (i%c == 0 && i in units[..index]);
+        {
+            if units[index]%c == 0 { results := results + [units[index]]; }
+            index := index + 1;
+        }
+    }
 }
 
 // Main method for testing functionality of BloodBank class
@@ -100,6 +125,7 @@ method Main() {
     // Initialise blood bank and index variables
     var bank: BloodBank;
     var i1: int, i2: int, i3: int, i4: int, i5: int;
+    var f1: seq<int>, f2: seq<int>;
 
     // Test 1: Tests functionality of AddUnit, FindUnitIndex and RemoveUnitByIndex
     bank := new BloodBank();
@@ -113,6 +139,8 @@ method Main() {
     bank.AddUnit(4); assert bank.units == [1,4];
     bank.AddUnit(2); assert bank.units == [1,4,2];
     bank.AddUnit(3); assert bank.units == [1,4,2,3];
+    f1 := bank.FilterUnits(2); assert 2 in f1 && 4 in f1 && 1 !in f1 && 3 !in f1;
+    f2 := bank.FilterUnits(3); assert 3 in f2 && 1 !in f2 && 2 !in f2 && 4 !in f2;
     i2 := bank.FindUnitIndex(2); assert bank.units[i2] == 2;
     i3 := bank.FindUnitIndex(3); assert bank.units[i3] == 3;
     i4 := bank.FindUnitIndex(4); assert bank.units[i4] == 4;
